semantics/ffi/ffiScript.sml
@@ -176,46 +176,52 @@ val _ = Define `
   )
 `
 
-(*
-val _ = Hol_datatype `
-  strval = Strv  of 'a
-         | Locv  of 'b  `;
-
-
-val _ = Hol_datatype `
-  cval = Boolv of bool
-       | Intv  of int
-       | Listv  of ('a,'b) strval `;
-*)
-
-val _ = Hol_datatype `
-  ar_str = Arr
-         | Str`;
-
-val _ = Define `
-   (get_carg (C_array conf) (C_arrayv ws) (SOME Str) = if conf.mutable then NONE else SOME (C_arrayv ws))
-/\ (get_carg (C_array conf) (C_arrayv ws) (SOME Arr) = if conf.mutable then SOME (C_arrayv ws) else NONE)
-/\ (get_carg C_bool (C_primv(C_boolv b))  NONE = SOME (C_primv (C_boolv b)))
-/\ (get_carg C_int  (C_primv(C_intv n))   NONE = SOME  (C_primv(C_intv n)))
-/\ (get_carg _ _ _ = NONE)`
-
-
-val _ = Define
-  `(get_cargs [] [] [] = SOME [])
-/\ (get_cargs (ty::tys) (arg::args) (tag::tags)=
-     OPTION_MAP2 CONS (get_carg ty arg tag) (get_cargs tys args tags))
-/\ (get_cargs _ _ _ = NONE)`
-
 val _ = Hol_datatype `
  outcome = Success | Resource_limit_hit | FFI_outcome of final_event`;
 
-(* should we remove args altogether? *)
+
+val get_cargs_def = Define
+  `(get_cargs _ [] [] = SOME [])
+/\ (get_cargs vcv (ty::tys) (arg::args) =
+    OPTION_MAP2 CONS (vcv ty arg) (get_cargs vcv tys args))
+/\ (get_cargs _ _ _ = NONE)
+`
+
+val store_cargs_def = Define
+  `(store_cargs s _ [] [] = SOME s)
+/\ (store_cargs s strf (marg::margs) (w::ws) =
+     case strf s marg w of
+        | SOME s' => store_cargs s' strf margs ws
+        | NONE => NONE)
+/\ (store_cargs s _ _ _ = SOME s)
+`
+
+
 val do_ffi_def = Define `
-  do_ffi ffi name vs tags =
+  do_ffi (st:'a) ffi store strf vcv name args =
     case FIND (\x.x.mlname = name) (debug_sig::ffi.signatures) of
       | SOME sign =>
-        let cts = sign.args; alsargs = als_args cts vs; mutargs = get_mut_args cts vs in
-        (case get_cargs cts vs tags of
+        let cts = sign.args; alsargs = als_args cts args; mutargs = get_mut_args cts args in
+        (case get_cargs vcv cts args of
+	  | SOME cargs =>
+            (case call_FFI ffi name sign cargs alsargs of
+              | SOME (FFI_return ffi' newargs retv) =>
+                (case store_cargs store strf mutargs newargs of
+                  | SOME str' => SOME (INR (ffi', str', retv))
+	          | NONE => NONE)
+              | SOME (FFI_final outcome) => SOME (INL outcome)
+                  | NONE => NONE)
+	  | NONE => NONE)
+      | NONE => NONE`
+
+
+(*
+val do_ffi_def = Define `
+  do_ffi (st:'a) ffi name vcv args =
+    case FIND (\x.x.mlname = name) (debug_sig::ffi.signatures) of
+      | SOME sign =>
+        let cts = sign.args; alsargs = als_args cts args; mutargs = get_mut_args cts args in
+        (case get_cargs vcv cts args of
 	  | SOME cargs =>
             (case call_FFI ffi name sign cargs alsargs of
               | SOME (FFI_return ffi' newargs retv) =>  SOME (INR (ffi', mutargs, retv, newargs))
@@ -223,8 +229,7 @@ val do_ffi_def = Define `
               | NONE => NONE)
 	  | NONE => NONE)
       | NONE => NONE`
-
-
+*)
 
 (*
 val do_ffi_def = Define `
@@ -240,7 +245,6 @@ val do_ffi_def = Define `
               | NONE => NONE)
 	  | NONE => NONE)
       | NONE => NONE`
-
 *)
 
 (* A program can Diverge, Terminate, or Fail. We prove that Fail is
